src/tls/PNE.fst
@@ -1,0 +1,84 @@
+module PNE
+
+module HST = FStar.HyperStack.ST
+module HS = FStar.HyperStack
+
+module I = Crypto.Indexing
+module U32 = FStar.UInt32
+module U128 = FStar.UInt128
+
+
+open FStar.HyperStack
+open FStar.Seq
+open FStar.Monotonic.Seq
+open FStar.Error
+open FStar.Bytes
+
+open FStar.Bytes
+open FStar.UInt32
+open Mem
+open Pkg
+
+    
+let table_region = new_region tls_region
+
+let tbl_ref (r:erid) (i:I.id) (u:info) : Tot Type0 =
+  m_rref r (Seq.seq (entry i u)) grows
+
+noeq type pne_state (i:I.id) (u:info) =
+  | PNE_state :
+    region: subrgn table_region ->
+    key: lbytes 16 ->  
+    tbl: tbl_ref region i u ->
+    pne_state i u
+
+let table (#i:I.id) (#u:info) (st:pne_state i u) (h:mem) : GTot (Seq.seq (entry i u)) =
+  sel h (PNE_state?.tbl st)
+
+
+let footprint (#i:I.id) (#u:info) (st:pne_state i u) =
+  PNE_state?.region st
+ 
+
+let create (i:I.id) (u:info) =
+  let rg = new_region table_region in
+  let k = CoreCrypto.random 16 in
+  let t = ralloc #(Seq.seq (entry i u)) #grows rg Seq.empty in
+  PNE_state rg k t
+
+//todo use the real aes/chacha from evercrypt
+assume val aes: lbytes 16 -> lbytes 16 -> lbytes 16
+
+#reset-options "--z3rlimit 50"
+
+let encrypt #i #u st n c =
+  let s = sample_cipher c in
+  let t = PNE_state?.tbl st in
+  let k = PNE_state?.key st in
+  let l = U32.uint_to_t pnlen in
+  if safePNE i then
+    (let ne = CoreCrypto.random pnlen in
+    t := Seq.snoc (!t) (Entry s ne n);
+    ne)
+  else
+    (let mask = Bytes.slice (aes k s) 0ul l in
+    let ne = Bytes.xor l (repr i u n) mask in
+    t := Seq.snoc (!t) (Entry s ne n);
+    ne)
+  
+
+let decrypt #i #u st ne c =
+  let s = sample_cipher c in
+  let t = PNE_state?.tbl st in
+  let k = PNE_state?.key st in
+  let l = U32.uint_to_t pnlen in
+  if safePNE i then
+    (match Seq.find_l (sample_filter i u s) !t with
+          | None -> None
+          | Some (Entry _ ne' n) -> 
+            if ne = ne' then Some n
+            else None)
+  else
+    (let mask = Bytes.slice (aes k s) 0ul l in
+    let n = Bytes.xor l ne mask in
+    Some (abs i u n))
