src/tls/PNE.fsti
@@ -1,0 +1,117 @@
+module PNE
+module HS = FStar.HyperStack
+
+module I = Crypto.Indexing
+module U32 = FStar.UInt32
+module U128 = FStar.UInt128
+
+open FStar.HyperStack
+open FStar.Seq
+open FStar.Monotonic.Seq
+open FStar.Error
+open FStar.Bytes
+
+open FStar.Bytes
+open FStar.UInt32
+open Mem
+open Pkg
+
+
+let pnlen = 4
+
+val table_region : rgn
+
+let safePNE (i:I.id) = Flag.safePNE i
+
+type cipher = b:bytes{Bytes.length b >= 16}
+
+type ciphersample = lbytes 16
+
+type epn = lbytes pnlen
+
+noeq type pn_pkg =
+  | PNPkg:
+    pn: (i:I.id -> (t:Type0{hasEq t})) ->
+    as_bytes: (i:I.id -> pn i -> GTot (lbytes pnlen)) ->
+    repr: (i:I.id{~(safePNE i)} -> n:pn i -> Tot (b:lbytes pnlen{b == as_bytes i n})) ->
+    from_bytes: (i:I.id -> b:lbytes pnlen -> GTot (n:pn i{as_bytes i n == b})) ->
+    abs: (i:I.id{~(safePNE i)} -> b:lbytes pnlen -> Tot (n:pn i{n == from_bytes i b})) ->
+    pn_pkg
+
+let info = pn_pkg
+
+let pn (i:I.id) (u:info) = PNPkg?.pn u i
+
+let repr (i:I.id{~(safePNE i)}) (u:info) (n:pn i u) = PNPkg?.repr u i n
+
+let abs (i:I.id{~(safePNE i)}) (u:info) (b:lbytes pnlen) = PNPkg?.abs u i b
+
+type entry (i:I.id) (u:info) =
+  | Entry :
+    s:ciphersample ->
+    ne:epn ->
+    n:pn i u ->
+    entry i u
+
+val pne_state : i:I.id -> u:info -> Type0
+
+val table : (#i:I.id) -> (#u:info) -> (st:pne_state i u) -> (h:mem) -> GTot (Seq.seq (entry i u))
+
+val footprint : #i:I.id -> #u:info -> st:pne_state i u -> GTot (subrgn table_region)
+ 
+let sample_filter (i:I.id) (u:info) (s:ciphersample) (e:entry i u) : bool =
+  Entry?.s e = s
+
+let entry_for_sample (#i:I.id) (#u:info) (s:ciphersample) (st:pne_state i u) (h:mem) :
+  GTot (option (entry i u)) =
+  Seq.find_l (sample_filter i u s) (table st h)
+  
+let fresh_sample (#i:I.id) (#u:info) (s:ciphersample) (st:pne_state i u) (h:mem) :
+  GTot bool =
+  None? (entry_for_sample s st h)
+
+let sample_cipher (c:cipher) : s:ciphersample =
+  Bytes.slice c 0ul 16ul
+
+val create (i:I.id) (u:info) : ST (pne_state i u)
+  (requires fun _ -> True)
+  (ensures fun h0 st h1 ->
+    modifies_none h0 h1 /\
+    table st h1 == Seq.empty)
+
+val encrypt :
+  (#i:I.id) ->
+  (#u:info) ->
+  (st:pne_state i u) ->
+  (n:pn i u) ->
+  (c:cipher) ->
+  ST epn
+  (requires fun h0 ->
+    fresh_sample (sample_cipher c) st h0)
+  (ensures fun h0 ne h1 ->
+    modifies_one (footprint st) h0 h1 /\
+    (let s = sample_cipher c in
+    table st h1 == Seq.snoc (table st h0) (Entry s ne n)))
+
+val decrypt :
+  (#i:I.id) ->
+  (#u: info) ->
+  (st:pne_state i u) ->
+  (ne:epn) ->
+  (c:cipher) ->
+  ST (option (pn i u))
+  (requires fun h0 -> True)
+  (ensures fun h0 on h1 ->
+    modifies_none h0 h1 /\
+    (let s = sample_cipher c in
+      (safePNE i ==>
+        (match entry_for_sample s st h0 with
+          | None -> None? on
+          | Some (Entry _ ne' n) -> 
+            if ne = ne' then on = Some n
+            else None? on)
+      )
+    )
+  )
+  
+
